\newcommand{\distance}{24em}
\newcommand{\classwidth}{4em}

\begin{tikzpicture}

\umlclassvarwidth{person}{}{Person}{
firstname\\
lastname
}{\classwidth}
\umlclassvarwidth[, right=\distance of person.north, anchor=north]{resident}{}{Resident}{
name
}{\classwidth}
\umlclassvarwidth[, below right=0.4*\distance and 0.5*\distance of person.north, anchor=north]{employee}{}{Employee}{
name
}{\classwidth}

\draw[consistency relation] 
    ([yshift=-2.0em]person.north east)
    --
    node[pos=0, above right] {$p$}
    node[pos=1, above left] {$r$}
    node[below, align=center] {$\{\tupled{p,r} \mid \mathvariable{r.name} = \mathvariable{p.firstname} + \textnormal{"\textvisiblespace"} + \mathvariable{p.lastname} $\\
    $\lor \mathvariable{r.name} = \mathvariable{p.lastname} + \textnormal{",\textvisiblespace"} + \mathvariable{p.firstname}\}$}
    ([yshift=-2.0em]resident.north west);
\draw[consistency relation] 
    ([xshift=0.7em]person.south)
    |-
    node[pos=0, below left] {$p$}
    node[pos=1, below left] {$e$}
    node[right, pos=0.35, align=center] {$\{\tupled{p,e} \mid\mathvariable{e.name} = \mathvariable{p.firstname} + \textnormal{"\textvisiblespace"} + \mathvariable{p.lastname} $\\
    $\lor \mathvariable{e.name} = \mathvariable{p.lastname} + \textnormal{"\textvisiblespace"} + \mathvariable{p.firstname} \}$}
    ([yshift=0.7em]employee.west);
\draw[consistency relation] 
    ([xshift=-0.7em]resident.south)
    |-
    node[pos=0, below right] {$r$}
    node[pos=1, below right] {$e$}
    node[left, pos=0.22, align=center] {$\{\tupled{e,r} \mid \mathvariable{r.name} = \mathvariable{e.name}\}$}
    ([yshift=0.7em]employee.east);

\draw[transformation, -latex] 
    ([yshift=-0.8em]person.north east)
    --
    node[above=0.5em, align=center] {
        $+p \rightarrow r(\mathvariable{name} = \mathvariable{p.lastname} + \textnormal{",\textvisiblespace}" + \mathvariable{p.firstname})$\\[0.2em]
        $\begin{aligned}
            \mathtextspaceafter{\textup{Alternative 1:}} \;
            +r \rightarrow p(
            &
                \mathvariable{firstname} = \mathvariable{r.name.substringAfter}(\textnormal{"\textvisiblespace"})\\
            &
                \mathvariable{lastname} = \mathvariable{r.name.substringBeforeFirst}(\textnormal{","}, \textnormal{"\textvisiblespace"})
            )\\
            \mathtextspaceafter{\textup{Alternative 2:}}
            +r \rightarrow \mathvariable{if}(
            &
                \mathvariable{r.name.contains}(\textnormal{","})) \mathtextspacearound{then Alternative 1, else} \\
            p(
            &
                \mathvariable{firstname} = \mathvariable{r.name.substringBefore}(\textnormal{"\textvisiblespace"}) \\
            &
                \mathvariable{lastname} = \mathvariable{r.name.substringAfter}(\textnormal{"\textvisiblespace"})
            )
        \end{aligned}$
    }
    ([yshift=-0.8em]resident.north west);
\draw[transformation, -latex] 
    ([xshift=-0.7em]person.south)
    |-
    node[below left=0.5em and 2.3em, pos=0.5, anchor=north west, align=center] {
        $\begin{aligned}
            +p \rightarrow +e(
            &
                \mathvariable{name} = \mathvariable{p.lastname} + \textnormal{"\textvisiblespace"} + \mathvariable{p.firstname}
            ) \\
            +e \rightarrow +p(
            &
                \mathvariable{firstname} = \mathvariable{e.name.substringAfter}(\textnormal{"\textvisiblespace"})\\
            &
                \mathvariable{lastname} = \mathvariable{e.name.substringBefore}(\textnormal{"\textvisiblespace"})
            )
        \end{aligned}$
    }
    ([yshift=-0.7em]employee.west);
\draw[transformation, latex-]
    ([xshift=0.7em]resident.south)
    |-
    node[below right=0.5em and 2.3em, pos=0.5, anchor=north east, align=center] {
        $+e \rightarrow +r(\mathvariable{name} = \mathvariable{e.name})$\\
        $+r \rightarrow +e(\mathvariable{name} = \mathvariable{r.name})$
    }
    ([yshift=-0.7em]employee.east);


\node[consistency preservation element, below=5em of employee.south, anchor=north] {
    $\begin{aligned}
    \mathtextspaceafter{\textup{with:}} \;
    & 
    \mathvariable{x.substringBefore}(\mathvariable{separator}) \equalsperdefinition \mathvariable{x.substring}(0, \mathvariable{x.indexOf}(\mathvariable{separator}))\\
    & 
    \mathvariable{x.substringBeforeFirst}(\mathvariable{separator1}, \mathvariable{separator2}) \equalsperdefinition\\
    &
    \formulaskip \mathvariable{x.substring}(\mathvariable{min}(\mathvariable{x.indexOf}(\mathvariable{separator1}), \mathvariable{x.indexOf}(\mathvariable{separator2})))\\
    & 
    \mathvariable{x.substringAfter}(\mathvariable{separator}) \equalsperdefinition \mathvariable{x.substring}(\mathvariable{x.indexOf}(\mathvariable{separator}) + 1)\\
    \end{aligned}$
};

\end{tikzpicture}